IntroEffects/SmallStep.lean
@@ -82,6 +82,7 @@ inductive Step : Computation → Computation → Prop
 -/
 | handleOpMiss h op v body (hop : h.lookup op = none) :
   Step (.handle (.hdl h) (.opCall op v body)) (opCall op v (.handle (.hdl h) body))
+| join s₁ s₂ : Step (.join (.string s₁) (.string s₂)) (.ret (.string (s₁ ++ " " ++ s₂)))
 
 infix:50 " ⤳ " => Step
 
