Main.lean
@@ -1,10 +1,30 @@
 import IntroEffects
 
--- Examples
+/-!
+  Examples of the language and its output after being evaluated.
+-/
 open Input
 
+def printFullName := {{{
+  do _a ← print(str("What is your forename?"); fun y ↦ (return y)) in
+  do forename ← read((); fun y ↦ (return y)) in
+  do _b ← print(str("What is your surname?"); fun y ↦ (return y)) in
+  do surname ← read((); fun y ↦ (return y)) in
+  do joined ← join(forename, surname) in
+  return joined
+}}}
+
 def alwaysRead := {{{
-  fun s ↦ (return handler {ops := ["read"(x,k) ↦ k s]})
+  fun s ↦ (return handler {ops := ["read"(x,k) ↦ k s, "print"(x,k) ↦ k ()]})
+}}}
+
+/--
+info: Bob Bob
+-/
+#guard_msgs in
+#evalLang {{{
+  do h ← ~alwaysRead str("Bob")  in
+  with h handle ~printFullName
 }}}
 
 def main : IO Unit :=
